Denote/Ex2.lean
@@ -1,0 +1,26 @@
+import Denote.PCF.Denote
+import Denote.PCF.Red
+
+/- ii) P (Topic 5-8): 2, 6, 8;  -/
+/-     L: 15, 17, 19 -/
+
+open PCF Dom
+
+def Ωi Γ t : ITerm Γ t := .fix <| .lam <| .var <| .hd
+
+theorem Nat.repeat.id {x : Nat} : x.repeat id = (id : A → A) := by 
+  induction x
+  · rfl
+  · simp_all only [Nat.repeat]; rfl
+
+theorem ex15 {Γ Δ} : (Ωi Γ t).denote Δ = ⊥ := by
+  change complete (Nat.repeat id · ⊥) _ = ⊥
+  conv => lhs; lhs; intro x; rw [Nat.repeat.id]; dsimp
+  rw [complete_const]
+
+example {Γ Δ arg t} : (ITerm.lam (Ωi (arg :: Γ) t)).denote Δ = (Ωi _ _).denote Δ := by
+  dsimp [ITerm.denote, CFunc.curry]
+  conv => lhs; lhs; intro x; rw [ex15]
+  rw [ex15]
+  rfl
+
