Denote/PCF/Denote.lean
@@ -1,0 +1,58 @@
+import Denote.PCF.Stx
+import Denote.PCF.DenoteDefs
+import Denote.Domain.Flat
+import Denote.Domain.FuncDom
+import Denote.Domain.DomConstructs
+
+namespace PCF
+
+open Dom
+
+instance {x : Sigma Dom} : Dom x.fst := x.snd
+
+noncomputable section
+
+@[simp]
+def Ty.denote' : Ty → Sigma Dom
+  | .arr t1 t2 => ⟨Dom.CFunc t1.denote'.fst t2.denote'.fst, inferInstance⟩
+  | .bool => ⟨Dom.Flat Bool, inferInstance⟩
+  | .nat => ⟨Dom.Flat Nat, inferInstance⟩
+
+@[simp]
+def Ty.denote : Ty → Type _ := Sigma.fst ∘ Ty.denote'
+
+instance {ty : Ty} : Dom ty.denote := ty.denote'.snd
+
+def ctx_denote : List Ty → Type _
+  | [] => PUnit
+  | hd :: tl => ctx_denote tl × hd.denote
+
+instance ctx_denote.isDom : {ls : List Ty} → Dom (ctx_denote ls)
+  | [] => (inferInstance : Dom PUnit)
+  | _ :: tl => 
+    have : Dom (ctx_denote tl) := isDom
+    (inferInstance : Dom (_ × _))
+
+def proj {ty} : {ctx : List _} → List.MemT ty ctx → CFunc (ctx_denote ctx) ty.denote
+  | _, .hd => .snd
+  | _, .tl h => .comp (proj h) .fst
+
+def ITerm.denote {ctx ty} : ITerm ctx ty → CFunc (ctx_denote ctx) ty.denote
+  | .var v => proj v
+  | .app t1 t2 => .comp .mp (.corecP t1.denote t2.denote)
+  | .lam f => .curry f.denote
+  | .true => .const (.obj .true)
+  | .false => .const (.obj .false)
+  | .zero => .const (.obj .zero)
+  | .succ v => succ.denote.comp v.denote
+  | .pred v => pred.denote.comp v.denote
+  | .fix v => .comp .fix v.denote
+  | .z? v => z?.denote.comp v.denote
+  | .ite c t f => ite.denote.comp
+      <| .corecP c.denote
+      <| .corecP t.denote f.denote
+
+end
+
+end PCF
+
