Denote/PCF/Red.lean
@@ -1,0 +1,52 @@
+import Denote.PCF.Stx
+
+namespace PCF
+
+def Term'.subst : Term' (Term' A) t → Term' A t
+  | .lam l => .lam fun v => (l (.var v)).subst
+  | .var v => v
+  | .app a b => .app a.subst b.subst
+
+  | .zero => .zero
+  | .false => .false
+  | .true => .true
+
+  | .succ v => .succ v.subst
+  | .fix v => .fix v.subst
+  | .z? v => .z? v.subst
+  | .pred v => .pred v.subst
+
+  | .ite c t f => .ite c.subst t.subst f.subst
+
+inductive Term'.Val : Term' A t → Prop
+  | zero : Val .zero
+  | succ : Val v → Val (.succ v)
+  | true : Val .true
+  | false : Val .false
+  | lam : Val (.lam l)
+
+def Term.Val (v : Term t) : Prop := 
+  Term'.Val (A := fun _ => PUnit) v
+
+inductive Red : Term t → Term t → Prop
+  | val : Term.Val v → Red v v
+  | succ : Red x v → Red (Term.succ x) (Term.succ v)
+  | pred : Red x (Term.succ v) → Red (Term.pred x) v
+  | z?z : Red x .zero → Red (Term.z? x) .true
+  | z?s : Red x (Term.succ _) → Red (Term.z? x) .false
+  | itet : Red c .true → Red t v → Red (Term.ite c t f) v
+  | itef : Red c .false → Red f v → Red (Term.ite c t f) v
+  | app {t : Term (.arr A B)} {u : Term A} {v : Term B} {f : {rep : Ty → Type} → rep A → Term B}
+      : Red t (Term.lam f) → Red (f u).subst v → Red (Term.app t u) v
+  | fix : Red (Term.app t (Term.fix t)) v → Red (Term.fix t) v
+
+theorem Red.rhs_Val (h : Red a b) : Term.Val b := by
+  induction h
+  any_goals assumption
+  case succ ih => exact .succ ih
+  case pred ih => cases ih; assumption
+  case z?z => exact .true
+  case z?s => exact .false
+
+def Ω (t : Ty) : Term t := .fix <| .lam fun x => .var x
+
